rename `Common.state` to `common_state`

thys/Real_Time_Deque/Common.thy
@@ -13,7 +13,7 @@ text \<open>
 \<^noindent> Each phase contains a \<open>current\<close> state, that holds the original elements of the deque end.
 \<close>
 
-datatype (plugins del: size)'a state = 
+datatype (plugins del: size)'a common_state = 
       Copy "'a current" "'a list" "'a list" nat
     | Idle "'a current" "'a idle"
 
@@ -24,7 +24,7 @@ text\<open>
 \<^descr> \<open>step\<close>: Executes one step of the transformation, while keeping the invariant.\<close>
 
 (* TODO: Maybe inline function? *)
-fun normalize :: "'a state \<Rightarrow> 'a state" where
+fun normalize :: "'a common_state \<Rightarrow> 'a common_state" where
   "normalize (Copy current old new moved) = (
     case current of Current extra added _ remained \<Rightarrow> 
       if moved \<ge> remained
@@ -33,10 +33,10 @@ fun normalize :: "'a state \<Rightarrow> 'a state" where
   )"
 
 
-instantiation state ::(type) step
+instantiation common_state ::(type) step
 begin
 
-fun step_state :: "'a state \<Rightarrow> 'a state" where
+fun step_common_state :: "'a common_state \<Rightarrow> 'a common_state" where
   "step (Idle current idle) = Idle current idle"
 | "step (Copy current aux new moved) = (
     case current of Current _ _ _ remained \<Rightarrow>
@@ -50,12 +50,12 @@ fun step_state :: "'a state \<Rightarrow> 'a state" where
 instance..
 end
 
-fun push :: "'a \<Rightarrow> 'a state \<Rightarrow> 'a state" where
+fun push :: "'a \<Rightarrow> 'a common_state \<Rightarrow> 'a common_state" where
   "push x (Idle current (idle.Idle stack stackSize)) = 
       Idle (Current.push x current) (idle.Idle (Stack.push x stack) (Suc stackSize))"
 | "push x (Copy current aux new moved) = Copy (Current.push x current) aux new moved"
 
-fun pop :: "'a state \<Rightarrow> 'a * 'a state" where
+fun pop :: "'a common_state \<Rightarrow> 'a * 'a common_state" where
   "pop (Idle current idle) = (let (x, idle) = Idle.pop idle in (x, Idle (drop_first current) idle))"
 | "pop (Copy current aux new moved) = 
       (first current, normalize (Copy (drop_first current) aux new moved))"
