thys/Real_Time_Deque/Common_Aux.thy
@@ -14,19 +14,19 @@ text\<open>
 definition take_rev where 
 [simp]:  "take_rev n xs = rev (take n xs)"
 
-fun list :: "'a state \<Rightarrow> 'a list" where
+fun list :: "'a common_state \<Rightarrow> 'a list" where
   "list (Idle _ idle) = Idle_Aux.list idle"
 | "list (Copy (Current extra _ _ remained) old new moved) 
    = extra @ take_rev (remained - moved) old @ new"
 
-fun list_current :: "'a state \<Rightarrow> 'a list" where
+fun list_current :: "'a common_state \<Rightarrow> 'a list" where
   "list_current (Idle current _) = Current_Aux.list current"
 | "list_current (Copy current _ _ _) = Current_Aux.list current"
 
-instantiation state::(type) invar
+instantiation common_state::(type) invar
 begin
 
-fun invar_state :: "'a state \<Rightarrow> bool" where
+fun invar_common_state :: "'a common_state \<Rightarrow> bool" where
   "invar (Idle current idle) \<longleftrightarrow>
       invar idle 
     \<and> invar current 
@@ -45,30 +45,30 @@ fun invar_state :: "'a state \<Rightarrow> bool" where
 instance..
 end
 
-instantiation state::(type) size
+instantiation common_state::(type) size
 begin
 
-fun size_state :: "'a state \<Rightarrow> nat" where
+fun size_common_state :: "'a common_state \<Rightarrow> nat" where
   "size (Idle current idle) = min (size current) (size idle)"
 | "size (Copy current _ _ _) = min (size current) (size_new current)"
 
 instance..
 end
 
-instantiation state::(type) size_new
+instantiation common_state::(type) size_new
 begin
 
-fun size_new_state :: "'a state \<Rightarrow> nat" where
+fun size_new_common_state :: "'a common_state \<Rightarrow> nat" where
   "size_new (Idle current _) = size_new current"
 | "size_new (Copy current _ _ _) = size_new current"
 
 instance..
 end
 
-instantiation state::(type) remaining_steps
+instantiation common_state::(type) remaining_steps
 begin
 
-fun remaining_steps_state :: "'a state \<Rightarrow> nat" where
+fun remaining_steps_common_state :: "'a common_state \<Rightarrow> nat" where
   "remaining_steps (Idle _ _) = 0"
 | "remaining_steps (Copy (Current _ _ _ remained) aux new moved) = remained - moved"
 
